basic stlc

TypeTheory/Stlc.lean
@@ -1,3 +1,7 @@
+import Mathlib.Data.Finmap
+
+set_option diagnostics.threshold 100
+
 namespace STLC
 
 inductive ty : Type :=
@@ -12,43 +16,272 @@ inductive tm : Type :=
   | tm_false : tm
   | tm_if : tm → tm → tm → tm
 
-notation "≪" e "≫" => e
-infixr:50  "→" => fun S T => ty.Ty_Arrow S T
-infixl:1   "↠" => fun S T => tm.tm_app S T
-notation:90 "λ" x:99 ":" t:99 "," y:99 => tm.tm_abs x t y
+notation " <{" e "}> " => (e : tm)
+infixr:50  " → " => ty.Ty_Arrow
+infixl:1   " ↠ " => tm.tm_app
+notation "BOOL" => ty.Ty_Bool
+notation:90 " λ " x:99 ": " t:99 ", " y:99 => tm.tm_abs x t y
 notation "If" x "Then" y "Else" z => tm.tm_if x y z
 notation "TRUE" => tm.tm_true
 notation "FALSE" => tm.tm_false
 
-#check ≪ tm.tm_var "x" ≫ ↠ ≪ tm.tm_abs "x" ty.Ty_Bool ≪tm.tm_var "x"≫ ≫
-#check ≪ tm.tm_var "x" ≫
-#check ≪ tm.tm_abs "x" ty.Ty_Bool ≪tm.tm_var "x"≫ ≫
-#check ≪ λ "x" : ty.Ty_Bool , tm.tm_var "x" ≫
+instance : Coe String tm := ⟨tm.tm_var⟩
+instance : Coe Bool tm := ⟨
+  fun b => match b with
+  | true => tm.tm_true
+  | false => tm.tm_false
+⟩
+
+example : <{true}> = TRUE := rfl
+example : <{false}> = FALSE := rfl
+
+def x : String := "x"
+def y : String := "y"
+def z : String := "z"
+
+#check (x : tm)
+#check <{x}>
+#check λ x: BOOL, x
+#check λ x: BOOL, x ↠ y ↠ z
+#check λ x: (BOOL → BOOL → BOOL), x ↠ x
+#check TRUE
 
 inductive value : tm → Prop
   | v_abs (x : String) (T : ty) (t : tm) :
-      value ≪ tm.tm_abs x T t ≫
-  | v_true : value ≪ tm.tm_true ≫
-  | v_false : value ≪ tm.tm_false ≫
+      value <{ λ x:T,t }>
+  | v_true : value <{ TRUE }>
+  | v_false : value <{ FALSE }>
 
 def subst (x : String) (s : tm) (t : tm) : tm :=
   match t with
   | tm.tm_var y =>
-    if x == y then s else t
+    if x = y then s else t
   | tm.tm_app t1 t2 =>
     (subst x s t1) ↠ (subst x s t2)
-  | tm.tm_abs y T t1 =>
-    if x == y then t else λ y: T, (subst x s t1)
-  | tm.tm_if t1 t2 t3 =>
-    If ≪subst x s t1≫ Then
-      ≪subst x s t2≫
-    Else
-      ≪subst x s t3≫
-  | tm.tm_true => TRUE
-  | tm.tm_false => FALSE
+  | λ y: T, t1 =>
+    if x = y then t else λ y: T, (subst x s t1)
+  | If t1 Then t2 Else t3 =>
+    If <{subst x s t1}> Then <{subst x s t2}>
+    Else <{subst x s t3}>
+  | TRUE => TRUE
+  | FALSE => FALSE
 
-notation t "[" x ":=" s "]" => subst x s t
+notation t " [" x ":=" s "] " => subst x s t
+
+#check <{λ x: BOOL, x}> [x := TRUE]
+
+example: <{λ x: BOOL, y}> [x := TRUE] = λ x: BOOL, y :=
+  rfl
+example: <{λ x: BOOL, y}> [y := TRUE] = λ x: BOOL, TRUE :=
+  rfl
+example: <{If x Then TRUE Else FALSE}> [x := TRUE] =
+          <{If true Then true Else false}> := rfl
+example: <{x ↠ x}> [x := (λ x: BOOL, x ↠ x)] =
+        <{(λ x: BOOL, x ↠ x) ↠ (λ x: BOOL, x ↠ x)}> := by
+  rfl
+
+inductive substi (s : tm) (x : String) : tm → tm → Prop :=
+  | s_var1 :
+    substi s x <{x}> s
+  | s_var2 (y : String) :
+    x ≠ y → substi s x <{y}> <{y}>
+  | s_app (t1 t2 t1' t2' : tm) :
+    substi s x t1 t1' → substi s x t2 t2' →
+    substi s x (t1 ↠ t2) (t1' ↠ t2')
+  | s_abs1 (T : ty) (t : tm) :
+    substi s x (λ x: T, t) (λ x: T, t)
+  | s_abs2 (y : String) (T : ty) (t t' : tm) :
+    x ≠ y → substi s x t t' →
+    substi s x (λ y: T, t) (λ y: T, t')
+  | s_true : substi s x TRUE TRUE
+  | s_false : substi s x FALSE FALSE
+  | s_if (t1 t2 t3 t1' t2' t3' : tm) :
+    substi s x t1 t1' → substi s x t2 t2' → substi s x t3 t3' →
+    substi s x (If t1 Then t2 Else t3) (If t1' Then t2' Else t3')
+
+open substi
+
+theorem substi_correct: ∀ s x t t', substi s x t t' ↔ t [x := s] = t' := by
+  intro s x t t'
+  constructor
+  · intro h
+    induction h with
+    | s_var1 =>
+      unfold subst
+      rw [if_pos rfl]
+    | s_var2 y h1 =>
+      unfold subst
+      rw [if_neg h1]
+    | s_app t1 t2 t1' t2' h1 h2 ih1 ih2 =>
+      unfold subst
+      rw [ih1, ih2]
+    | s_abs1 T t =>
+      unfold subst
+      rw [if_pos rfl]
+    | s_abs2 y T t t' h1 h2 ih =>
+      unfold subst
+      rw [if_neg h1, ih]
+    | s_true => rfl
+    | s_false => rfl
+    | s_if t1 t2 t3 t1' t2' t3' h1 h2 h3 ih1 ih2 ih3 =>
+      unfold subst
+      rw [ih1, ih2, ih3]
+  . intro h
+    induction t generalizing x s t' with
+    | tm_var y =>
+      rw [← h]; unfold subst
+      cases (decEq x y) with
+      | isTrue h => rw [if_pos h]; exact h ▸ s_var1
+      | isFalse h => rw [if_neg h]; exact s_var2 y h
+    | tm_app t1 t2 ih1 ih2 =>
+      rw [← h]; unfold subst
+      apply s_app
+      · apply ih1; rfl
+      · apply ih2; rfl
+    | tm_abs y T t ih =>
+      rw [← h]; unfold subst
+      cases (decEq x y) with
+      | isTrue h => rw [if_pos h]; exact h ▸ s_abs1 T t
+      | isFalse h =>
+        rw [if_neg h]
+        apply s_abs2 y T t
+        · exact h
+        · apply ih; rfl
+    | tm_true => exact h ▸ s_true
+    | tm_false => exact h ▸ s_false
+    | tm_if t1 t2 t3 ih1 ih2 ih3 =>
+      rw [← h]; unfold subst
+      apply s_if
+      · apply ih1; rfl
+      · apply ih2; rfl
+      · apply ih3; rfl
+
+inductive step : tm → tm → Prop :=
+  | ST_AppAbs : ∀ x T2 t1 v2,
+    value v2 → step <{(λ x: T2, t1) ↠ v2}> <{t1 [x := v2]}>
+  | ST_App1 : ∀ t1 t1' t2,
+    step t1 t1' → step <{t1 ↠ t2}> <{t1' ↠ t2}>
+  | ST_App2 : ∀ v1 t2 t2',
+    value v1 → step t2 t2' → step <{v1 ↠ t2}> <{v1 ↠ t2'}>
+  | ST_IfTrue : ∀ t1 t2,
+    step <{If TRUE Then t1 Else t2}> t1
+  | ST_IfFalse : ∀ t1 t2,
+    step <{If FALSE Then t1 Else t2}> t2
+  | ST_If : ∀ t1 t1' t2 t3,
+    step t1 t1' → step <{If t1 Then t2 Else t3}> <{If t1' Then t2 Else t3}>
+
+notation x " -> " y => step x y
+inductive multi {X : Type} (R : X → X → Prop) : X → X → Prop
+  | multi_refl : ∀ x, multi R x x
+  | multi_step : ∀ x y z, R x y → multi R y z → multi R x z
+open multi
+notation "multistep" => multi step
+notation x " ->* " y => multistep x y
+
+def idBB := <{λ x: (BOOL → BOOL), x}>
+def idB := <{λ x: BOOL, x}>
+def idBBBB := <{λ x: ((BOOL → BOOL) → (BOOL → BOOL)), x}>
+def K := <{λ x: BOOL, <{λ y: BOOL, x}> }>
+def notB := <{λ x: BOOL, If x Then FALSE Else TRUE}>
 
 
+#check (idBB ↠ idB)
+#check idB
+
+example : <{idBB ↠ idB}> ->* idB := by
+  apply multi_step
+  · apply step.ST_AppAbs
+    apply value.v_abs
+  apply multi_refl
+
+example : <{ idBB ↠ <{idBB ↠ idB}>}> ->* idB := by
+  apply multi_step
+  --  <{ idBB ↠ <{idBB ↠ idB}>}>  ->  <{idBB ↠ idB}>
+  · apply step.ST_App2
+    · apply value.v_abs
+    · apply step.ST_AppAbs
+      apply value.v_abs
+  -- <{idBB ↠ idB}>  ->*  idB
+  apply multi_step
+  · apply step.ST_AppAbs
+    apply value.v_abs
+  apply multi_refl
+
+example : <{ idBB ↠ notB ↠ TRUE}> ->* FALSE := by
+  apply multi_step
+  · apply step.ST_App1;
+    apply step.ST_AppAbs
+    apply value.v_abs
+  apply multi_step
+  · apply step.ST_AppAbs
+    apply value.v_true
+  dsimp [subst]
+  apply multi_step
+  · apply step.ST_IfTrue
+  apply multi_refl
+
+example : <{ idBB ↠ (notB ↠ TRUE) }> ->* <{FALSE}> := by
+  sorry
+
+example : <{ idBBBB ↠ idBB ↠ idB }> ->* idB := by
+  sorry
+
+
+def context := Finmap (fun _:String => ty)
+instance : EmptyCollection context:= ⟨(∅ : Finmap (fun _:String => ty))⟩
+#check (∅ : context)
+
+open Finmap
+inductive has_type : context → tm → ty → Prop :=
+  | T_Var : ∀ Gamma x T1,
+    (Finmap.lookup x Gamma) = some T1 →
+      has_type Gamma <{x}> T1
+  | T_Abs : ∀ Gamma x T1 T2 t1,
+    has_type (Gamma.insert x T1) t1 T2 →
+      has_type Gamma <{λ x: T1, t1}> (T1 → T2)
+  | T_app : ∀ Gamma t1 t2 T1 T2,
+    has_type Gamma t1 (T1 → T2) →
+    has_type Gamma t2 T1 →
+    has_type Gamma <{t1 ↠ t2}> T2
+  | T_True : ∀ Gamma,
+    has_type Gamma <{TRUE}> BOOL
+  | T_False : ∀ Gamma,
+    has_type Gamma <{FALSE}> BOOL
+  | T_If : ∀ Gamma t1 t2 t3 T,
+    has_type Gamma t1 BOOL →
+    has_type Gamma t2 T →
+    has_type Gamma t3 T →
+    has_type Gamma <{If t1 Then t2 Else t3}> T
+open has_type
+
+notation Gamma " ⊢ " t " : " T => has_type Gamma t T
+set_option diagnostics true
+#check ∅ ⊢ x : BOOL
+#check  ∅ ⊢ (λ x: BOOL, x) : BOOL → BOOL
+example : ∅ ⊢ λ x: BOOL, x : BOOL → BOOL := by
+  apply T_Abs
+  apply T_Var
+  rfl
+
+example : ∅ ⊢ λ x: BOOL, <{λ y : (BOOL → BOOL), (y ↠ (y ↠ x))}> : BOOL → (BOOL → BOOL) → BOOL := by
+  apply T_Abs
+  apply T_Abs
+  apply T_app
+  · apply T_Var
+    rfl
+  apply T_app
+  · apply T_Var
+    rfl
+  apply T_Var
+  rfl
+
+example : ∃ T, ∅ ⊢ λ x : (BOOL → BOOL), <{λ y : (BOOL → BOOL), <{λ z : BOOL, (y ↠ (x ↠ z))}>}> : T := by
+  sorry
+
+example : ¬ ∃ T, ∅ ⊢ λ x : BOOL, <{λ y : BOOL, (x ↠ y)}> : T := by
+  sorry
+
+example : ¬ (∃ S T, ∅ ⊢ λ x : S, <{y ↠ y}> : T) := by
+  sorry
 
 end STLC
